coq/TypedSyntaxProperties.v
@@ -2,7 +2,7 @@
 Require Import Koika.TypedSyntaxFunctions Koika.TypedSemantics.
 
 Section TypedSyntaxProperties.
-  Context {pos_t var_t rule_name_t reg_t ext_fn_t: Type}.
+  Context {pos_t var_t fn_name_t rule_name_t reg_t ext_fn_t: Type}.
   Context {reg_t_eq_dec: EqDec reg_t}.
 
   Context {R: reg_t -> type}.
@@ -12,8 +12,8 @@ Section TypedSyntaxProperties.
   Context (r: REnv.(env_t) R).
   Context (sigma: forall f, Sig_denote (Sigma f)).
 
-  Notation rule := (rule pos_t var_t R Sigma).
-  Notation action := (action pos_t var_t R Sigma).
+  Notation rule := (rule pos_t var_t fn_name_t R Sigma).
+  Notation action := (action pos_t var_t fn_name_t R Sigma).
   Notation scheduler := (scheduler pos_t rule_name_t).
   Notation Log := (Log R REnv).
 
@@ -30,57 +30,56 @@ Section TypedSyntaxProperties.
 
   Ltac dec_step :=
     match goal with
+    | _ => progress intros
     | _ => eassumption || discriminate || reflexivity
     | _ => bool_step || cleanup_step
     | _ => progress (cbn in *; subst)
     | [ H: False |- _ ] => destruct H
     | [ H: Some _ = Some _ |- _ ] => inversion H; subst; clear H
-    | [ H: context[let/opt _ := ?x in _] |- _ ] => destruct x eqn:?
-    | [  |- context[if ?x then _ else _] ] => destruct x eqn:?
-    | _ => solve [eauto]
+    | [ H: context[let/opt _ := ?x in _] |- _ ] =>
+      destruct x as [ ((? & ?) & ?) | ] eqn:?
+    | [  |- context[if ?x then _ else _] ] =>
+      destruct x eqn:?
+    | [ H: context[if ?x then _ else _] |- _ ] =>
+      destruct x eqn:?
+    | [ H: Some _ = Some _ |- _ ] => inversion H; subst; clear H
+    | _ => solve [intuition eauto 3 using bits_to_N_zero]
     end.
 
   Lemma returns_zero_correct {sig tau} :
     forall (a: action sig tau) (Gamma: tcontext sig) (sched_log: Log) (action_log: Log),
       returns_zero a = true ->
-      match interp_action r sigma Gamma sched_log action_log a with
-      | Some (_, v, _) => bits_of_value v = Bits.zeroes (type_sz tau)
-      | None => True
-      end.
+      forall l v G,
+        interp_action r sigma Gamma sched_log action_log a = Some (l, v, G) ->
+        bits_of_value v = Bits.zeroes (type_sz tau).
   Proof.
-    induction a; cbn; intros; try discriminate;
-      repeat match goal with
-             | _ => dec_step
-             | [ H: (forall Gamma L l, _ -> match interp_action ?r ?sigma Gamma L l ?a with _ => _ end)
-                 |- context[interp_action ?r ?sigma ?Gamma ?L ?l ?a] ] =>
-               specialize (H Gamma L l)
-             | [ H: returns_zero ?x = true -> _, H': returns_zero ?x = true |- _ ] =>
-               specialize (H H')
-             | [  |- context[opt_bind (interp_action ?r ?sigma ?Gamma ?sched_log ?action_log ?a) _] ] =>
-               destruct (interp_action r sigma Gamma sched_log action_log a) as [ ((? & ?) & ?) | ]
-             | _ => eauto using bits_to_N_zero || simpl
-             end.
+    induction a; repeat dec_step.
   Qed.
 
-  Lemma is_pure_correct {sig tau} :
-    forall (a: action sig tau) (Gamma: tcontext sig) (sched_log: Log) (action_log: Log),
+  Lemma is_pure_correct :
+    forall {sig tau} (a: action sig tau) (Gamma: tcontext sig) (sched_log: Log) (action_log: Log),
       is_pure a = true ->
-      match interp_action r sigma Gamma sched_log action_log a with
-      | Some (l, _, _) => l = action_log
-      | None => False
-      end.
+      forall l l' v G,
+        l = l' ->
+        interp_action r sigma Gamma sched_log action_log a = Some (l', v, G) ->
+        l = action_log.
   Proof.
-    induction a; cbn; intros; try discriminate;
-    repeat match goal with
-           | _ => dec_step
-           | [ H: (forall Gamma sched_log action_log,
-                      _ -> match interp_action ?r ?sigma Gamma sched_log action_log ?a with
-                          | _ => _ end) |-
-               context[interp_action ?r ?sigma ?Gamma ?sched_log ?action_log ?a] ] =>
-             specialize (H Gamma sched_log action_log ltac:(eauto));
-               destruct (interp_action r sigma Gamma sched_log action_log a)
-               as [ ((? & ?) & ?) | ] eqn:?
-           end.
+    fix IH 3; destruct a; repeat dec_step.
+    assert (forall l l' v G,
+               l = l' ->
+               interp_args r sigma Gamma sched_log action_log args = Some (l', v, G) ->
+               l = action_log).
+
+    { clear dependent a; clear t t2 Heqo.
+      revert dependent Gamma.
+      revert dependent sched_log.
+      revert dependent action_log.
+      revert dependent argspec.
+      fix IHargs 2; destruct args; cbn; intros;
+        repeat dec_step. }
+
+    etransitivity; [ eapply IH | ].
+    all: eauto.
   Qed.
 
   Lemma action_type_correct {sig tau} (a: action sig tau):
@@ -91,14 +90,14 @@ Section TypedSyntaxProperties.
     forall (a: action sig tau) (Gamma: tcontext sig) (sched_log: Log) (action_log: Log),
       is_tt a = true ->
       tau = unit_t /\
-      match interp_action r sigma Gamma sched_log action_log a with
-      | Some (_, v, _) => bits_of_value v = Bits.zeroes (type_sz tau)
-      | None => False
-      end.
+      forall l v G,
+       interp_action r sigma Gamma sched_log action_log a = Some (l, v, G) ->
+       bits_of_value v = Bits.zeroes (type_sz tau).
   Proof.
-    unfold is_tt; intros.
+    unfold is_tt;
     repeat match goal with
            | _ => dec_step
+           | [  |- _ /\ _ ] => split
            | [ H: vect_nil_t _ |- _ ] => destruct H
            | [ H: context[beq_dec] |- _ ] => rewrite beq_dec_iff in H
            | [ H: context[action_type _] |- _ ] => apply action_type_correct in H
@@ -112,21 +111,15 @@ Section TypedSyntaxProperties.
   Lemma interp_arithmetic_correct {sig tau} :
     forall (a: action sig tau) (Gamma: tcontext sig) (sched_log: Log) (action_log: Log) res,
       interp_arithmetic a = Some res ->
-      match interp_action r sigma Gamma sched_log action_log a with
-      | Some (_, v, _) => v = res
-      | None => False
-      end.
+      forall l v G,
+      interp_action r sigma Gamma sched_log action_log a = Some (l, v, G) ->
+      v = res.
   Proof.
-    induction a; cbn; intros;
-    repeat match goal with
-           | _ => dec_step
-           | [ H: (forall Gamma sched_log action_log _,
-                      _ -> match interp_action ?r ?sigma Gamma sched_log action_log ?a with
-                          | _ => _ end) |-
-               context[interp_action ?r ?sigma ?Gamma ?sched_log ?action_log ?a] ] =>
-             specialize (H Gamma sched_log action_log _ ltac:(eauto));
-               destruct (interp_action r sigma Gamma sched_log action_log a)
-               as [ ((? & ?) & ?) | ] eqn:?
-           end.
+    induction a;
+      repeat match goal with
+             | _ => dec_step
+             | [ H: context[opt_bind ?x] |- _ ] => destruct x
+             | _ => f_equal
+             end.
   Qed.
 End TypedSyntaxProperties.
